eval apply machine generation

refocusing_signatures.v
@@ -303,3 +303,65 @@ Module Type STAGED_ABSTRACT_MACHINE (R : RED_LANG).
   | e_intro : forall {t k} {v : value k}, dec t [_] v -> eval t v.
 
 End STAGED_ABSTRACT_MACHINE.
+
+
+
+Module Type EVAL_APPLY_MACHINE (R : RED_LANG).
+
+  Import R.
+
+  (** Functions specifying atomic steps of induction on terms and contexts -- needed to avoid explicit induction on terms and contexts in construction of the AM *)
+  Parameter dec_term    : term -> forall k, interm_dec k.
+  Parameter dec_context : forall ec k, value (k+>ec) -> interm_dec k.
+
+  Axiom dec_term_correct : 
+      forall t k, match dec_term t k with
+      | in_red r       => t = r
+      | in_val v       => t = v
+      | in_term t0 ec0 => t = ec0:[t0]
+      | in_dead        => dead_ckind k
+      end.
+
+  Axiom dec_context_correct : 
+      forall ec k v, match dec_context ec k v with
+      | in_red r      => ec:[v] = r
+      | in_val v0     => ec:[v] = v0
+      | in_term t ec0 => ec:[v] = ec0:[t]
+      | in_dead       => dead_ckind (k+>ec) 
+      end.
+
+
+  Inductive dec : term -> forall {k1 k2}, context k1 k2 -> value k1 -> Prop :=
+  | d_d_r  : forall t {t0 k1 k2} {c : context k1 k2} {r v},
+               dec_term t k2 = in_red r -> contract r = Some t0 -> dec t0 c v ->
+               dec t c v
+  | d_v    : forall t {k1 k2} {c : context k1 k2} {v v0},
+               dec_term t k2 = in_val v -> decctx v c v0 ->
+               dec t c v0
+  | d_term : forall t {t0 ec k1 k2} {c : context k1 k2} {v},
+               dec_term t k2 = in_term t0 ec -> dec t0 (ec=:c) v ->
+               dec t c v
+
+  with decctx : forall {k2}, value k2 -> forall {k1}, context k1 k2 -> value k1 -> Prop :=
+  | dc_end : forall {k} (v : value k), 
+               ~ dead_ckind k ->
+               decctx v [_] v
+  | dc_red : forall ec {k2} (v : value (k2+>ec)) {k1} {c : context k1 k2} {r t v0},
+               dec_context ec k2 v = in_red r -> contract r = Some t -> dec t c v0 ->
+               decctx v (ec=:c) v0
+  | dc_rec : forall ec {k2} (v : value (k2+>ec)) {k1} {c : context k1 k2} {v0 v1},
+               dec_context ec k2 v = in_val v0 -> decctx v0 c v1 ->
+               decctx v (ec=:c) v1
+  | dc_trm : forall ec {k2} (v : value (k2+>ec)) {k1} {c : context k1 k2} {t ec0 v0},
+               dec_context ec k2 v = in_term t ec0 -> dec t (ec0=:c) v0 ->
+               decctx v (ec=:c) v0.
+
+
+  Scheme dec_Ind := Induction for dec Sort Prop
+    with decctx_Ind := Induction for decctx Sort Prop.
+
+
+  Inductive eval : term -> forall {k}, value k -> Prop :=
+  | e_intro : forall {t k} {v : value k}, dec t [_] v -> eval t v.
+
+End EVAL_APPLY_MACHINE.
